Prove Reaction.Output.events_LawfulQueue (assuming Array.map_getElem?)

Runtime/Network/Execution/Apply.lean
@@ -2,37 +2,43 @@ import Runtime.Network.Execution.Basic
 
 open Network
 
-structure Reaction.Output (net : Network) where
+structure Reaction.Output (exec : Executable net) where
   reactor : ReactorId net
   reaction : reactor.class.reactionType
-  time : Time
-  raw : reaction.outputType time
+  raw : reaction.outputType exec.tag.time
 
-abbrev Reaction.Output.domain (output : Reaction.Output net) : Interface.Scheme :=
+abbrev Reaction.Output.domain (output : Reaction.Output exec) : Interface.Scheme :=
   output.reactor.class.interface .outputs
 
-def Reaction.Output.fromRaw {reactor : ReactorId net} {reaction : reactor.class.reactionType} {time} (raw : reaction.outputType time) : Reaction.Output net :=
-  { reactor, reaction, time, raw }
+variable {exec : Executable net}
 
-def Reaction.Output.events (output : Reaction.Output net) :=
+def Reaction.Output.fromRaw {reactor : ReactorId net} {reaction : reactor.class.reactionType} (raw : reaction.outputType exec.tag.time) : Reaction.Output exec :=
+  { reactor, reaction, raw }
+
+def Reaction.Output.events (output : Reaction.Output exec) :=
   output.raw.events.map fun event => Event.action event.time ⟨output.reactor, event.action⟩ event.value
 
-inductive Reaction.Output.LocalValue (output : Reaction.Output net) (port : output.domain.vars)
+inductive Reaction.Output.LocalValue (output : Reaction.Output exec) (port : output.domain.vars)
   | independent
   | absent
-  | present (value : output.domain.type port) -- {port : output.reaction.portEffects} (value : (output.reactor.class.interface .outputs).restrict output.reaction.portEffects |>.type port)
+  | present (value : output.domain.type port)
+
+inductive Reaction.Output.NestedValue (output : Reaction.Output exec) (port : output.domain.vars)
+  | independent
+  | absent
+  | present (value : output.domain.type port) 
 
 def Reaction.Output.LocalValue.value? : LocalValue output port → Option (output.domain.type port)
   | present value        => value
   | independent | absent => none
 
 -- Note: This theorem is really only needed for `Reaction.Output.local`.
-def Reaction.Output.local_type_correctness {port'} : 
+private def Reaction.Output.local_type_correctness {port'} : 
   (output.reaction.portEffectsInjCoe.inv (.inl port) = some port') → 
   (output.reactor.class.reactionOutputScheme |>.restrict output.reaction.portEffects |>.type port') = (domain output).type port :=
   (by rw [Interface.Scheme.restrict_type, output.reaction.portEffectsInjCoe.invCoeId _ ·])
 
-def Reaction.Output.local (output : Reaction.Output net) (port : output.domain.vars) : LocalValue output port := 
+def Reaction.Output.local (output : Reaction.Output exec) (port : output.domain.vars) : LocalValue output port := 
   match h : output.reaction.portEffectsInjCoe.inv (.inl port) with
   | none => .independent
   | some port' =>
@@ -40,29 +46,38 @@ def Reaction.Output.local (output : Reaction.Output net) (port : output.domain.v
     | none => .absent
     | some value => .present (local_type_correctness h ▸ value)
 
+theorem Reaction.Output.events_LawfulQueue (output : Reaction.Output exec) : Executable.LawfulQueue output.events exec.tag.time := by
+  intro event h
+  simp [events, Array.map_getElem?, Bind.bind, Option.bind] at h
+  split at h
+  · contradiction
+  case _ e _ => 
+    simp at h
+    simp [Event.time, ←h, e.time.property]
+
 namespace Network.Executable    
 
-def apply (exec : Executable net) (output : Reaction.Output net) : Executable net := { exec with
+def apply (exec : Executable net) (output : Reaction.Output exec) : Executable net := { exec with
   queue := exec.queue.merge output.events
   reactors := fun id => { exec.reactors id with
     interface := 
-      if      h : id = output.reactor then h ▸ targetReactor exec output  -- Updates the output ports of the reaction's reactor.
-      else if h : id ≻ output.reactor then nestedReactor exec output id h -- Updates the input ports of nested reactors.
+      if      h : id = output.reactor then h ▸ targetReactor output  -- Updates the output ports of the reaction's reactor.
+      else if h : id ≻ output.reactor then nestedReactor output id h -- Updates the input ports of nested reactors.
       else                                 exec.reactors id |>.interface  -- Unaffected reactors.
   }
-  lawfulQueue := sorry
+  lawfulQueue := LawfulQueue.merge exec.lawfulQueue output.events_LawfulQueue
 }
 where 
-  targetReactor (exec : Executable net) (output : Reaction.Output net) : (kind : Reactor.InterfaceKind) → kind.interfaceType (output.reactor.class.interface kind)
+  targetReactor (output : Reaction.Output exec) : (kind : Reactor.InterfaceKind) → kind.interfaceType (output.reactor.class.interface kind)
     | .outputs => fun var => (output.local var).value?.orElse (fun _ => exec.interface output.reactor .outputs var)
     | .state => output.raw.state
     | interface => exec.interface output.reactor interface
-  nestedReactor (exec : Executable net) (output : Reaction.Output net) (id : ReactorId net) (hc : id ≻ output.reactor) : (kind : Reactor.InterfaceKind) → kind.interfaceType (id.class.interface kind)
-    | .inputs => nestedInputs exec output id hc
+  nestedReactor (output : Reaction.Output exec) (id : ReactorId net) (hc : id ≻ output.reactor) : (kind : Reactor.InterfaceKind) → kind.interfaceType (id.class.interface kind)
+    | .inputs => sorry -- nestedInputs exec output id hc
     | interface => exec.reactors id |>.interface interface 
-  nestedInputs (exec : Executable net) (output : Reaction.Output net) (id : ReactorId net) (hc : id ≻ output.reactor) : Interface? (id.class.interface .inputs) :=
-    let currentReactor := exec.reactors id
-    fun var =>
+  -- nestedInputs (exec : Executable net) (output : Reaction.Output net) (id : ReactorId net) (hc : id ≻ output.reactor) : Interface? (id.class.interface .inputs) :=
+  --  let currentReactor := exec.reactors id
+  --  fun var =>
       /-
       let nestedID := id.last hc
       have h₁ : (net.scheme id |>.interface .inputs).vars = (net.subinterface (net.class reactorID) nestedID .inputs).vars := by sorry -- rw [Graph.child_schemes_eq_parent_subschemes]
@@ -80,7 +95,6 @@ where
             sorry
           h ▸ val
       -/
-      sorry
 
 
 end Network.Executable    
